theories/MetaTheory/Conversion.v
@@ -5,7 +5,7 @@ From Metaprog.MetaTheory Require Export Confluence.
     and develops the equational theory of [conv]. *)
 
 (***********************************************************************)
-(** * Conversion relation [conv]. *)
+(** * Conversion relation on terms. *)
 (***********************************************************************)
 
 Reserved Notation "Γ ⊢ t ≡ u"
@@ -36,7 +36,7 @@ Lemma conv_of_red {s} Σ (t u : term s) :
 Proof.
 intros H. induction H.
 - reflexivity.
-- rewrite IHrefl_trans_clos. now apply conv_of_red1.
+- rewrite IHred. now apply conv_of_red1.
 Qed.
 
 #[export] Instance subrelation_red_conv s Σ :
@@ -54,18 +54,16 @@ Proof. intros t u H. unfold Basics.flip. symmetry. now apply conv_of_red. Qed.
 (** The Church-Rosser theorem is a direct consequence of the confluence lemma.
     We use Church-Rosser to prove inversion lemmas for [conv]. *)
 Lemma church_rosser {s} Σ (t1 t2 : term s) :
-  Σ ⊢ t1 ≡ t2 <->
+  Σ ⊢ t1 ≡ t2 ->
   exists u, Σ ⊢ t1 ~~> u /\ Σ ⊢ t2 ~~> u.
 Proof.
-split ; intros H.
-- depind H.
-  + exists t2. split ; [now apply red_of_red1 | reflexivity].
-  + exists t. now split.
-  + destruct IHconv as (u & H1 & H2). exists u. now split.
-  + destruct IHconv1 as (u1 & H1 & H2). destruct IHconv2 as (u2 & H3 & H4).
-    destruct (red_confluence Σ t2 u1 u2 H2 H3) as (u & H5 & H6).
-    exists u. split ; etransitivity ; eassumption.
-- destruct H as (u & H1 & H2). now rewrite H1, H2.
+intros H. depind H.
+- exists t2. split ; [now apply red_of_red1 | reflexivity].
+- exists t. now split.
+- destruct IHconv as (u & H1 & H2). exists u. now split.
+- destruct IHconv1 as (u1 & H1 & H2). destruct IHconv2 as (u2 & H3 & H4).
+  destruct (red_confluence Σ t2 u1 u2 H2 H3) as (u & H5 & H6).
+  exists u. split ; etransitivity ; eassumption.
 Qed.
 
 (***********************************************************************)
@@ -139,20 +137,6 @@ Section CongruenceLemmas.
   - apply conv_app_congr_aux with (l := []). assumption.
   Qed.
 
-  #[export] Instance conv_rename {s'} (ρ : ren s s') :
-    Proper (conv Σ ==> conv Σ) (rename ρ).
-  Proof.
-  intros t t' H. rewrite church_rosser in H. destruct H as (u & H1 & H2).
-  now rewrite H1, H2.
-  Qed.
-
-  #[export] Instance conv_substitute {s'} (σ : subst s s') :
-    Proper (conv Σ ==> conv Σ) (substitute σ).
-  Proof.
-  intros t t' H. rewrite church_rosser in H. destruct H as (u & H1 & H2).
-  now rewrite H1, H2.
-  Qed.
-
 End CongruenceLemmas.
 
 (***********************************************************************)
@@ -199,3 +183,120 @@ Section InversionLemmas.
   Qed.
 
 End InversionLemmas.
+
+(***********************************************************************)
+(** * Conversion relation on substitutions. *)
+(***********************************************************************)
+
+(** Conversion on substitutions is just pointwise conversion.
+    We wrap the definition in a record to avoid setoid rewrite issues. *)
+Record sconv {s s'} (Σ : evar_map) (σ σ' : subst s s') : Prop := {
+  sconv_prop : forall i, Σ ⊢ sapply σ i ≡ sapply σ' i
+}.
+
+#[export] Instance sconv_Reflexive s s' Σ : Reflexive (@sconv s s' Σ).
+Proof. intros σ. constructor. reflexivity. Qed.
+
+#[export] Instance sconv_Symmetric s s' Σ : Symmetric (@sconv s s' Σ).
+Proof. intros σ σ' [Hσ]. constructor. intros i. now symmetry. Qed.
+
+#[export] Instance sconv_Transitive s s' Σ : Transitive (@sconv s s' Σ).
+Proof.
+intros σ1 σ2 σ3 [H1] [H2]. constructor. intros i. etransitivity ; eauto.
+Qed.
+
+#[export] Instance conv_sapply {s s'} Σ :
+  Proper (sconv Σ ==> eq ==> conv Σ) (@sapply s s').
+Proof. intros σ σ' [Hσ] i ? <-. apply Hσ. Qed.
+
+#[export] Instance sconv_of_sred {s s'} Σ :
+  subrelation (@sred s s' Σ) (@sconv s s' Σ).
+Proof. intros σ σ' Hσ. constructor. intros i. now rewrite Hσ. Qed.
+
+#[export] Instance sconv_of_sred_flip {s s'} Σ :
+  subrelation (Basics.flip (@sred s s' Σ)) (@sconv s s' Σ).
+Proof. intros σ σ' Hσ. constructor. intros i. now rewrite Hσ. Qed.
+
+(** Church Rosser lemma on substitutions.
+    This is a simple consequence of the Church Rosser lemma on terms. *)
+Lemma church_rosser_subst {s s' Σ} (σ σ' : subst s s') :
+  sconv Σ σ σ' ->
+  exists τ, sred Σ σ τ /\ sred Σ σ' τ.
+Proof.
+revert s' σ σ'. induction s.
+- intros s' σ σ' Hσ. exists (sren wk_idx). split ; constructor ; intros i ; depelim i.
+- intros s' σ σ' Hσ.
+  specialize (IHs s' (rscomp rshift σ) (rscomp rshift σ')).
+  forward IHs. { constructor. intros i. simpl_subst. now rewrite Hσ. }
+  destruct IHs as (τ & H1 & H2).
+  assert (exists t, Σ ⊢ sapply σ I0 ~~> t /\ Σ ⊢ sapply σ' I0 ~~> t) as (t & Ht1 & Ht2).
+  { apply church_rosser. now rewrite Hσ. }
+  exists (scons x t τ). split.
+  + constructor. intros i. depelim i ; simpl_subst.
+    * exact Ht1.
+    * destruct H1 as [H1]. specialize (H1 i). simpl_subst in H1. exact H1.
+  + constructor. intros i. depelim i ; simpl_subst.
+    * exact Ht2.
+    * destruct H2 as [H2]. specialize (H2 i). simpl_subst in H2. exact H2.
+Qed.
+
+(***********************************************************************)
+(** * Compatibility of conversion with substitution. *)
+(***********************************************************************)
+
+#[export] Instance conv_rename {s s' Σ} (ρ : ren s s') :
+  Proper (conv Σ ==> conv Σ) (rename ρ).
+Proof.
+intros t t' H. apply church_rosser in H. destruct H as (u & H1 & H2).
+now rewrite H1, H2.
+Qed.
+
+#[export] Instance conv_substitute {s s' Σ} :
+  Proper (sconv Σ ==> conv Σ ==> conv Σ) (@substitute s s').
+Proof.
+intros σ σ' Hσ t t' Ht.
+apply church_rosser in Ht. destruct Ht as (u & -> & ->).
+apply church_rosser_subst in Hσ. destruct Hσ as (? & -> & ->).
+reflexivity.
+Qed.
+
+#[export] Instance conv_scons {s s' x Σ} :
+  Proper (conv Σ ==> sconv Σ ==> sconv Σ) (@scons s s' x).
+Proof.
+intros t t' Ht σ σ' Hσ. constructor. intros i.
+apply church_rosser in Ht. destruct Ht as (? & -> & ->).
+apply church_rosser_subst in Hσ. destruct Hσ as (? & -> & ->).
+reflexivity.
+Qed.
+
+#[export] Instance conv_srcomp {s s' x Σ} :
+  Proper (sconv Σ ==> eq ==> sconv Σ) (@srcomp s s' x).
+Proof.
+intros σ σ' Hσ ρ ρ' <-. constructor. intros i.
+apply church_rosser_subst in Hσ. destruct Hσ as (? & -> & ->).
+reflexivity.
+Qed.
+
+#[export] Instance conv_rscomp {s s' x Σ} :
+  Proper (eq ==> sconv Σ ==> sconv Σ) (@rscomp s s' x).
+Proof.
+intros ρ ρ' <- σ σ' Hσ. constructor. intros i.
+apply church_rosser_subst in Hσ. destruct Hσ as (? & -> & ->).
+reflexivity.
+Qed.
+
+#[export] Instance conv_sup {s s' x Σ} :
+  Proper (sconv Σ ==> sconv Σ) (@sup s s' x).
+Proof.
+intros σ σ' Hσ. apply church_rosser_subst in Hσ.
+destruct Hσ as (? & -> & ->). reflexivity.
+Qed.
+
+#[export] Instance conv_scomp {s s' x Σ} :
+  Proper (sconv Σ ==> sconv Σ ==> sconv Σ) (@scomp s s' x).
+Proof.
+intros σ σ' Hσ τ τ' Hτ. apply church_rosser_subst in Hσ, Hτ.
+destruct Hσ as (? & -> & ->). destruct Hτ as (? & -> & ->).
+reflexivity.
+Qed.
+
